pulse/ulib/experimental/Steel.Heap.fsti
@@ -188,6 +188,10 @@ val h_exists_cong (#a:Type) (p q : a -> slprop)
 val intro_h_exists (#a:_) (x:a) (p:a -> slprop) (h:heap)
   : Lemma (interp (p x) h ==> interp (h_exists p) h)
 
+(** Eliminate an existential by simply getting a proposition. *)
+val elim_h_exists (#a:_) (p:a -> slprop) (h:heap)
+  : Lemma (interp (h_exists p) h ==> (exists x. interp (p x) h))
+
 (**
   The interpretation of a separation logic proposition [hp] is itself an [hprop] of footprint
   [hp]
@@ -228,6 +232,18 @@ val pts_to_compatible
        (composable pcm v0 v1 /\
         interp (pts_to x (op pcm v0 v1)) h))
 
+(** If a reference points to two different values, they must be joinable
+in the PCM, even when the pointing does not happen separately. *)
+val pts_to_join (#a:Type u#a) (#pcm:_) (r:ref a pcm) (v1 v2:a) (m:heap)
+  : Lemma (requires (interp (pts_to r v1) m /\ interp (pts_to r v2) m))
+          (ensures joinable pcm v1 v2)
+
+(** Further, the value in the heap is a witness for that property *)
+val pts_to_join' (#a:Type u#a) (#pcm:_) (r:ref a pcm) (v1 v2:a) (m:heap)
+  : Lemma (requires (interp (pts_to r v1) m /\ interp (pts_to r v2) m))
+          (ensures (exists z. compatible pcm v1 z /\ compatible pcm v2 z /\
+                         interp (pts_to r z) m))
+
 val pts_to_compatible_equiv (#a:Type)
                             (#pcm:_)
                             (x:ref a pcm)
@@ -243,6 +259,15 @@ val intro_star (p q:slprop) (hp:hheap p) (hq:hheap q)
     : Lemma
       (requires disjoint hp hq)
       (ensures interp (p `star` q) (join hp hq))
+
+val elim_star (p q:slprop) (h:hheap (p `star` q))
+    : Lemma
+      (requires interp (p `star` q) h)
+    (ensures exists hl hr.
+      disjoint hl hr /\
+      h == join hl hr /\
+      interp p hl /\
+      interp q hr)
 
 (** [star] is commutative *)
 val star_commutative (p1 p2:slprop)
@@ -498,9 +523,40 @@ val change_slprop (p q:slprop)
 
 module U = FStar.Universe
 
+(** Implication of slprops *)
+let slimp (p1 p2:slprop) : prop =
+  forall m. interp p1 m ==> interp p2 m
+
+let is_frame_monotonic #a (p : a -> slprop) : prop =
+  forall x y m frame. interp (p x `star` frame) m /\ interp (p y) m ==> slimp (p x) (p y)
+
+let witness_invariant #a (p : a -> slprop) =
+  forall x y m. interp (p x) m /\ interp (p y) m ==> x == y
+
+val id_elim_star (p q:slprop) (h:heap)
+  : Pure (erased heap & erased heap )
+         (requires (interp (p `star` q) h))
+         (ensures (fun (hl, hr) -> disjoint hl hr
+                              /\ h == join hl hr
+                              /\ interp p hl
+                              /\ interp q hr))
+
+val id_elim_exists (#a:Type) (p : a -> slprop) (h:heap)
+  : Pure (erased a)
+         (requires (interp (h_exists p) h))
+         (ensures (fun x -> interp (p x) h))
+
+
+val witness_h_exists (#a:_) (p:a -> slprop{is_frame_monotonic p})
+  : action (h_exists p) (erased a) (fun x -> p x)
+
 val lift_h_exists (#a:_) (p:a -> slprop)
   : action (h_exists p) unit
            (fun _a -> h_exists #(U.raise_t a) (U.lift_dom p))
 
 val elim_pure (p:prop)
   : action (pure p) (u:unit{p}) (fun _ -> emp)
+
+val pts_to_evolve (#a:Type u#a) (#pcm:_) (r:ref a pcm) (x y : a) (h:heap)
+  : Lemma (requires (interp (pts_to r x) h /\ compatible pcm y x))
+          (ensures  (interp (pts_to r y) h))
