pulse/ulib/experimental/Steel.Memory.fst
@@ -41,6 +41,12 @@ let mem_of_heap (h:H.heap) : mem = {
   locks = []
 }
 
+let mem_set_heap (m:mem) (h:H.heap) : mem = {
+  ctr = m.ctr;
+  heap = h;
+  locks = m.locks;
+}
+
 let core_mem (m:mem) : mem = mem_of_heap (heap_of_mem m)
 
 let disjoint (m0 m1:mem u#h)
@@ -156,6 +162,22 @@ let pts_to_compatible_equiv #a #pcm v0 v1 = H.pts_to_compatible_equiv v0 v1
 
 let intro_star p q mp mq =
   H.intro_star p q (heap_of_mem mp) (heap_of_mem mq)
+
+let elim_star p q m =
+  let h = heap_of_mem m in
+  H.elim_star p q h;
+  assert (exists hl hr. H.disjoint hl hr /\ H.join hl hr == h /\ H.interp p hl /\ H.interp q hr);
+  let hl = FStar.IndefiniteDescription.indefinite_description_tot H.heap (fun hl ->
+     exists hr. H.disjoint hl hr /\ H.join hl hr == h /\ H.interp p hl /\ H.interp q hr) in
+  let hr = FStar.IndefiniteDescription.indefinite_description_tot H.heap (fun hr ->
+     H.disjoint hl hr /\ H.join hl hr == h /\ H.interp p hl /\ H.interp q hr) in
+  let ml = mem_set_heap m hl in
+  let mr = mem_set_heap m hr in
+  assert (disjoint ml mr);
+  assert (m == join ml mr);
+  assert (interp p ml);
+  assert (interp q mr);
+  ()
 
 let star_commutative (p1 p2:slprop) =
   H.star_commutative p1 p2
@@ -285,6 +307,8 @@ let h_exists_cong (#a:Type) (p q : a -> slprop)
       H.h_exists_cong p q
 
 let intro_h_exists #a x p m = H.intro_h_exists x p (heap_of_mem m)
+
+let elim_h_exists (#a:_) (p:a -> slprop) (m:mem) = H.elim_h_exists p (heap_of_mem m)
 
 ////////////////////////////////////////////////////////////////////////////////
 // Preorders and effects
@@ -1051,7 +1075,123 @@ let change_slprop (#opened_invariants:inames)
     in
     lift_tot_action (lift_heap_action opened_invariants (Steel.Heap.change_slprop p q proof))
 
+(* This module reuses is_frame_monotonic from Heap, but does not expose that
+to clients, so we need this lemma to typecheck witness_h_exists below. *)
+let relate_frame_monotonic_1 #a p
+  : Lemma (requires (H.is_frame_monotonic p))
+          (ensures (is_frame_monotonic p))
+  = ()
+
+let relate_frame_monotonic_2 #a p
+  : Lemma (requires (is_frame_monotonic p))
+          (ensures (H.is_frame_monotonic p))
+  =  let aux (x y : a) (h : H.heap) (f : H.slprop) :
+      Lemma (requires (H.interp (p x `H.star` f) h /\ H.interp (p y) h))
+            (ensures (H.slimp (p x) (p y)))
+      =
+        let m = mem_of_heap h in
+        assert (interp (p x `star` f) m);
+        assert (interp (p y)          m);
+        assert (slimp (p x) (p y));
+        let aux2 (h:H.heap) : Lemma (requires H.interp (p x) h) (ensures H.interp (p y) h) =
+          let m = mem_of_heap h in
+          assert (interp (p x) m);
+          assert (interp (p y) m);
+          ()
+        in
+        Classical.forall_intro (Classical.move_requires aux2)
+    in
+    Classical.forall_intro_4 (fun x y h f -> Classical.move_requires (aux x y h) f)
+
+let witness_h_exists #opened_invariants #a p =
+  relate_frame_monotonic_2 p;
+  lift_tot_action (lift_heap_action opened_invariants (H.witness_h_exists p))
 
 let lift_h_exists #opened_invariants p = lift_tot_action (lift_heap_action opened_invariants (H.lift_h_exists p))
 
 let elim_pure #opened_invariants p = lift_tot_action (lift_heap_action opened_invariants (H.elim_pure p))
+
+let pts_to_join (#a:Type) (#pcm:pcm a) (r:ref a pcm) (x y : a) (m:mem) :
+  Lemma (requires (interp (pts_to r x) m /\ interp (pts_to r y) m))
+        (ensures (joinable pcm x y)) =
+  H.pts_to_join r x y (heap_of_mem m)
+
+let pts_to_evolve (#a:Type u#a) (#pcm:_) (r:ref a pcm) (x y : a) (m:mem)
+  : Lemma (requires (interp (pts_to r x) m /\ compatible pcm y x))
+          (ensures  (interp (pts_to r y) m))
+  = H.pts_to_evolve r x y (heap_of_mem m)
+
+let id_elim_star p q m =
+  let starprop (ml:mem) (mr:mem) =
+      disjoint ml mr
+    /\ m == join ml mr
+    /\ interp p ml
+    /\ interp q mr
+  in
+  elim_star p q m;
+  let p1 : mem -> prop = fun ml -> (exists mr. starprop ml mr) in
+  let ml = IndefiniteDescription.indefinite_description_tot _ p1 in
+  let starpropml mr : prop = starprop ml mr in // this prop annotation seems needed
+  let mr = IndefiniteDescription.indefinite_description_tot _ starpropml in
+  (ml, mr)
+
+let id_elim_exists #a p m =
+  let existsprop (x:a) =
+    interp (p x) m
+  in
+  elim_h_exists p m;
+  let x = IndefiniteDescription.indefinite_description_tot _ existsprop in
+  x
+
+
+let slimp_star (p q r s : slprop)
+  : Lemma (requires (slimp p q /\ slimp r s))
+          (ensures (slimp (p `star` r) (q `star` s)))
+  = let aux (m:mem) : Lemma (requires (interp (p `star` r) m))
+                            (ensures (interp (q `star` s) m))
+    =
+      let (ml, mr) = id_elim_star p r m in
+      intro_star q s ml mr
+   in
+   Classical.forall_intro (Classical.move_requires aux)
+
+let elim_wi #a (p : a -> slprop{witness_invariant p}) (x y : a) (m : mem)
+  : Lemma (requires (interp (p x) m /\ interp (p y) m))
+          (ensures (x == y))
+  = ()
+
+let witinv_framon (#a:Type) (p : a -> slprop)
+  : Lemma (witness_invariant p ==> is_frame_monotonic p)
+          [SMTPatOr [[SMTPat (witness_invariant p)]; [SMTPat (is_frame_monotonic p)]]]
+  = ()
+
+let star_is_frame_monotonic (#a:Type)
+    (f g : a -> slprop)
+  : Lemma (requires (is_frame_monotonic f /\ is_frame_monotonic g))
+          (ensures (is_frame_monotonic (fun x -> f x `star` g x)))
+          //[SMTPat (is_frame_monotonic (fun x -> f x `star` g x))]
+  = let aux (x y : a) (m:mem) (frame : slprop)
+       : Lemma (requires interp ((f x `star` g x) `star` frame) m
+                        /\ interp (f y `star` g y) m)
+               (ensures (slimp (f x `star` g x) (f y `star` g y)))
+       = assert (slimp (f x) (f y));
+         star_associative (f x) (g x) frame;
+         Classical.forall_intro (affine_star (g x) frame);
+         assert (slimp (g x) (g y));
+         slimp_star (f x) (f y) (g x) (g y);
+         ()
+    in
+    Classical.forall_intro_4 (fun x y m -> Classical.move_requires (aux x y m));
+    ()
+
+let star_is_witinv_left (#a:Type)
+    (f g : a -> slprop)
+  : Lemma (requires (witness_invariant f))
+          (ensures  (witness_invariant (fun x -> f x `star` g x)))
+  = ()
+
+let star_is_witinv_right (#a:Type)
+    (f g : a -> slprop)
+  : Lemma (requires (witness_invariant g))
+          (ensures  (witness_invariant (fun x -> f x `star` g x)))
+  = ()
