pulse/ulib/experimental/Steel.Reference.fst
@@ -63,7 +63,7 @@ let hide_raise_reveal (#a:Type) (v0:erased a) (v1:erased a)
     assert (U.downgrade_val (U.raise_val (reveal v0)) == U.downgrade_val (U.raise_val (reveal v1)) <==>
             v0 == v1)
 
-let gather_atomic #a #uses #p0 #p1 #v0 #v1 r = 
+let gather_atomic #a #uses #p0 #p1 #v0 #v1 r =
   let x = H.gather_atomic r in
   A.return_atomic x
 
@@ -80,7 +80,7 @@ let downgrade_equiv (#t:Type) (x y:U.raise_t t)
   = assert (U.raise_val (U.downgrade_val x) == x);
     assert (U.raise_val (U.downgrade_val y) == y)
 
-let lift_eq (#t:eqtype) (x y:U.raise_t t) 
+let lift_eq (#t:eqtype) (x y:U.raise_t t)
   : b:bool{b <==> x==y}
   = downgrade_equiv x y; U.downgrade_val x = U.downgrade_val y
 
@@ -97,7 +97,7 @@ let cas_action (#t:eqtype)
             (pts_to r full_perm v)
             (fun b -> if b then pts_to r full_perm v_new else pts_to r full_perm v)
    = let hv =     (Ghost.hide (U.raise_val (Ghost.reveal v))) in
-     let b = H.cas_action #(U.raise_t t) 
+     let b = H.cas_action #(U.raise_t t)
                   (lift_eq #t)
                   #uses
                   r
@@ -117,3 +117,20 @@ let cas #t #uses r v v_old v_new = A.as_atomic_action (cas_action #t #uses r v v
 let raise_ref r p v = Basics.return r
 
 let lower_ref r p v = Basics.return r
+
+let pts_to_witinv (#a:Type u#0) (r:ref a) (p:perm)
+  : Lemma (witness_invariant  (pts_to r p))
+  = let aux (x y : erased a) (m : mem)
+      : Lemma (requires (interp (pts_to r p x) m
+                       /\ interp (pts_to r p y) m))
+              (ensures x == y)
+      = H.pts_to_witinv r p
+    in
+    Classical.forall_intro (fun x ->
+    Classical.forall_intro (fun y ->
+    Classical.forall_intro (fun m ->
+    Classical.move_requires (aux x y) m)))
+
+let pts_to_framon (#a:Type u#0) (r:ref a) (p:perm)
+  : Lemma (is_frame_monotonic (pts_to r p))
+  = pts_to_witinv r p
